\documentclass[a4paper,12pt]{article}
\usepackage[utf8x]{inputenc}
\usepackage{amssymb}
\usepackage{xlop}
\usepackage{xcolor}
\input{longdiv}
\usepackage{graphicx}
\usepackage{wrapfig}
\usepackage{float}
%PDF metadata
\usepackage[pdftex, 
pdfauthor={Juan Carlos Alvarez},
pdfsubject={matematicas},
pdfkeywords={matematicas}]{hyperref}
%opening
\hypersetup{pdftitle={Solucion prueva}}
\title{Soluci√≥n}
\author{}
\date{}
\begin{document}
\maketitle
Realiza las siguientes multiplicaciones: \vspace{1cm}\\ 
1)$(+7a)(+5y)=35ay $\vspace{1cm}\\ 
2)$(-8y)(-8e)=64ye $\vspace{1cm}\\ 
3)$(-3z)(-9p)=27zp $\vspace{1cm}\\ 
Realiza las siguientes multiplicaciones: \vspace{1cm}\\ 
4)$(+3w^{-2})(+6w^{-4} )=18w^{-6} $\vspace{1cm}\\ 
5)$(-3s^{-3})(-9s^{-5} )=27s^{-8} $\vspace{1cm}\\ 
6)$(-9l^{2})(+2l^{5} )=-18l^{7} $\vspace{1cm}\\ 
Realiza las siguientes multiplicaciones: \vspace{1cm}\\ 
7)$(-5w^{2})(+5d^{-4}+-9v^{-2} )= -25w^{2}d^{-4}45w^{2}v^{-2}   $\vspace{1cm}\\ 
8)$(-5i^{-4})(-9i^{2}++8n^{-3} )= 45i^{-2}-40i^{-4}n^{-3}   $\vspace{1cm}\\ 
9)$(+9x^{2})(-7l^{3}++9z^{-4} )= -63x^{2}l^{3}81x^{2}z^{-4}   $\vspace{1cm}\\ 
Realiza las siguientes multiplicaciones: \vspace{1cm}\\ 
10)$(+7b^{-4}-9e^{-4} )(-3f^{5}-3h^{2} )= -21b^{-4}f^{5}-21b^{-4}h^{2}+27e^{-4}f^{5}+27e^{-4}h^{2}$\vspace{1cm}\\ 
11)$(+9p^{4}-3u^{5} )(+7x^{-5}+6d^{-3} )= +63p^{4}x^{-5}+54p^{4}d^{-3}-21u^{5}x^{-5}-18u^{5}d^{-3}$\vspace{1cm}\\ 
12)$(+5b^{3}+7h^{3} )(+7v^{-2}+7w^{-3} )= +35b^{3}v^{-2}+35b^{3}w^{-3}+49h^{3}v^{-2}+49h^{3}w^{-3}$\vspace{1cm}\\ 

 \pagebreak 
Realiza las siguientes multiplicaciones: \vspace{1cm}\\ 
1)$(-2t)(-9k)=18tk $\vspace{1cm}\\ 
2)$(+2a)(+8c)=16ac $\vspace{1cm}\\ 
3)$(-7g)(+3z)=-21gz $\vspace{1cm}\\ 
Realiza las siguientes multiplicaciones: \vspace{1cm}\\ 
4)$(+9g^{4})(-5g^{2} )=-45g^{6} $\vspace{1cm}\\ 
5)$(-8j^{2})(-3j^{-2} )=24j^{0}=24 $\vspace{1cm}\\ 
6)$(-3a^{3})(+8a^{2} )=-24a^{5} $\vspace{1cm}\\ 
Realiza las siguientes multiplicaciones: \vspace{1cm}\\ 
7)$(-3a^{-2})(+8i^{-2}+-3t^{5} )= -24a^{-2}i^{-2}9a^{-2}t^{5}   $\vspace{1cm}\\ 
8)$(-6a^{3})(-3p^{-5}++2l^{-3} )= 18a^{3}p^{-5}-12a^{3}l^{-3}   $\vspace{1cm}\\ 
9)$(-4k^{4})(+3q^{4}+-6p^{3} )= -12k^{4}q^{4}24k^{4}p^{3}   $\vspace{1cm}\\ 
Realiza las siguientes multiplicaciones: \vspace{1cm}\\ 
10)$(-3c^{5}-7i^{4} )(-2k^{-2}-6l^{-4} )= +6c^{5}k^{-2}+18c^{5}l^{-4}+14i^{4}k^{-2}+42i^{4}l^{-4}$\vspace{1cm}\\ 
11)$(+8e^{3}+9g^{-2} )(+5m^{5}+7b^{5} )= +40e^{3}m^{5}+56e^{3}b^{5}+45g^{-2}m^{5}+63g^{-2}b^{5}$\vspace{1cm}\\ 
12)$(+8z^{4}+3s^{4} )(-6i^{-2}+2k^{3} )= -48z^{4}i^{-2}+16z^{4}k^{3}-18s^{4}i^{-2}+6s^{4}k^{3}$\vspace{1cm}\\ 

 \pagebreak 
Realiza las siguientes multiplicaciones: \vspace{1cm}\\ 
1)$(-9x)(+9u)=-81xu $\vspace{1cm}\\ 
2)$(+5b)(+8r)=40br $\vspace{1cm}\\ 
3)$(-5r)(+3x)=-15rx $\vspace{1cm}\\ 
Realiza las siguientes multiplicaciones: \vspace{1cm}\\ 
4)$(-4u^{5})(-9u^{-2} )=36u^{3} $\vspace{1cm}\\ 
5)$(-7z^{3})(-3z^{4} )=21z^{7} $\vspace{1cm}\\ 
6)$(+2y^{4})(+6y^{-3} )=12y $\vspace{1cm}\\ 
Realiza las siguientes multiplicaciones: \vspace{1cm}\\ 
7)$(+6h^{3})(+7k^{3}+-2d^{-3} )= 42h^{3}k^{3}-12h^{3}d^{-3}   $\vspace{1cm}\\ 
8)$(+8p^{-5})(+2t^{4}++7s^{4} )= 16p^{-5}t^{4}56p^{-5}s^{4}   $\vspace{1cm}\\ 
9)$(-3a^{2})(-6q^{-2}+-3l^{5} )= 18a^{2}q^{-2}9a^{2}l^{5}   $\vspace{1cm}\\ 
Realiza las siguientes multiplicaciones: \vspace{1cm}\\ 
10)$(+6c^{4}+8j^{4} )(+7y^{-2}+9o^{3} )= +42c^{4}y^{-2}+54c^{4}o^{3}+56j^{4}y^{-2}+72j^{4}o^{3}$\vspace{1cm}\\ 
11)$(-9x^{3}+6o^{-2} )(+2v^{-5}+8d^{2} )= -18x^{3}v^{-5}-72x^{3}d^{2}+12o^{-2}v^{-5}+48o^{-2}d^{2}$\vspace{1cm}\\ 
12)$(+8q^{2}-5g^{-5} )(+9r^{-4}+5h^{3} )= +72q^{2}r^{-4}+40q^{2}h^{3}-45g^{-5}r^{-4}-25g^{-5}h^{3}$\vspace{1cm}\\ 

 \pagebreak 
Realiza las siguientes multiplicaciones: \vspace{1cm}\\ 
1)$(-6b)(+9a)=-54ba $\vspace{1cm}\\ 
2)$(+9c)(-7l)=-63cl $\vspace{1cm}\\ 
3)$(-8i)(+8g)=-64ig $\vspace{1cm}\\ 
Realiza las siguientes multiplicaciones: \vspace{1cm}\\ 
4)$(+7e^{2})(+9e^{3} )=63e^{5} $\vspace{1cm}\\ 
5)$(+3e^{-5})(-4e^{3} )=-12e^{-2} $\vspace{1cm}\\ 
6)$(+5q^{-2})(+5q^{-4} )=25q^{-6} $\vspace{1cm}\\ 
Realiza las siguientes multiplicaciones: \vspace{1cm}\\ 
7)$(+8j^{-5})(+5g^{-2}+-7a^{-2} )= 40j^{-5}g^{-2}-56j^{-5}a^{-2}   $\vspace{1cm}\\ 
8)$(-5l^{-5})(+2z^{-4}+-6f^{5} )= -10l^{-5}z^{-4}30l^{-5}f^{5}   $\vspace{1cm}\\ 
9)$(-8b^{-4})(+3z^{-2}+-8q^{5} )= -24b^{-4}z^{-2}64b^{-4}q^{5}   $\vspace{1cm}\\ 
Realiza las siguientes multiplicaciones: \vspace{1cm}\\ 
10)$(+5v^{2}+7l^{2} )(-4h^{-2}+8y^{-5} )= -20v^{2}h^{-2}+40v^{2}y^{-5}-28l^{2}h^{-2}+56l^{2}y^{-5}$\vspace{1cm}\\ 
11)$(-6d^{5}+4j^{5} )(-4w^{3}+2o^{5} )= +24d^{5}w^{3}-12d^{5}o^{5}-16j^{5}w^{3}+8j^{5}o^{5}$\vspace{1cm}\\ 
12)$(-6j^{-5}-6c^{-3} )(-3i^{-3}-3h^{-2} )= +18j^{-5}i^{-3}+18j^{-5}h^{-2}+18c^{-3}i^{-3}+18c^{-3}h^{-2}$\vspace{1cm}\\ 

 \pagebreak 
Realiza las siguientes multiplicaciones: \vspace{1cm}\\ 
1)$(-7d)(-9v)=63dv $\vspace{1cm}\\ 
2)$(+8s)(+7u)=56su $\vspace{1cm}\\ 
3)$(-8i)(+3o)=-24io $\vspace{1cm}\\ 
Realiza las siguientes multiplicaciones: \vspace{1cm}\\ 
4)$(+2n^{5})(-5n^{2} )=-10n^{7} $\vspace{1cm}\\ 
5)$(+5c^{-3})(-7c^{4} )=-35c $\vspace{1cm}\\ 
6)$(-7a^{-5})(+9a^{2} )=-63a^{-3} $\vspace{1cm}\\ 
Realiza las siguientes multiplicaciones: \vspace{1cm}\\ 
7)$(-7w^{4})(-9y^{-2}+-2i^{-4} )= 63w^{4}y^{-2}14w^{4}i^{-4}   $\vspace{1cm}\\ 
8)$(+4c^{-5})(+8n^{2}++9q^{-5} )= 32c^{-5}n^{2}36c^{-5}q^{-5}   $\vspace{1cm}\\ 
9)$(+8u^{2})(-2v^{-3}+-5m^{-3} )= -16u^{2}v^{-3}-40u^{2}m^{-3}   $\vspace{1cm}\\ 
Realiza las siguientes multiplicaciones: \vspace{1cm}\\ 
10)$(+2r^{-4}-3j^{-5} )(-2n^{-3}+2c^{5} )= -4r^{-4}n^{-3}+4r^{-4}c^{5}+6j^{-5}n^{-3}-6j^{-5}c^{5}$\vspace{1cm}\\ 
11)$(-4n^{-2}-2b^{-4} )(+4v^{3}-9s^{-4} )= -16n^{-2}v^{3}+36n^{-2}s^{-4}-8b^{-4}v^{3}+18b^{-4}s^{-4}$\vspace{1cm}\\ 
12)$(+8x^{-2}+8f^{5} )(-9m^{4}-9z^{-5} )= -72x^{-2}m^{4}-72x^{-2}z^{-5}-72f^{5}m^{4}-72f^{5}z^{-5}$\vspace{1cm}\\ 

 \pagebreak 
\end{document}