\documentclass[a4paper,12pt]{article}
\usepackage[utf8x]{inputenc}
\usepackage{amssymb}
\usepackage{xlop}
\usepackage{xcolor}
\input{longdiv}
\usepackage{graphicx}
\usepackage{wrapfig}
\usepackage{float}
%PDF metadata
\usepackage[pdftex, 
pdfauthor={Juan Carlos Alvarez},
pdfsubject={matematicas},
pdfkeywords={matematicas}]{hyperref}
%opening
\hypersetup{pdftitle={Tarea prueva} }
\title{Tarea}
\author{}
\date{}
\begin{document}
\maketitle
Realiza las siguientes multiplicaciones: \vspace{1cm}\\ 
1)$(+7a)(+5y)=$\vspace{1cm}\\ 
2)$(-8y)(-8e)=$\vspace{1cm}\\ 
3)$(-3z)(-9p)=$\vspace{1cm}\\ 
Realiza las siguientes multiplicaciones: \vspace{1cm}\\ 
4)$(+3w^{-2})(+6w^{-4} )=$\vspace{1cm}\\ 
5)$(-3s^{-3})(-9s^{-5} )=$\vspace{1cm}\\ 
6)$(-9l^{2})(+2l^{5} )=$\vspace{1cm}\\ 
Realiza las siguientes multiplicaciones: \vspace{1cm}\\ 
7)$(-5w^{2})(+5d^{-4}+-9v^{-2} )=$\vspace{1cm}\\ 
8)$(-5i^{-4})(-9i^{2}++8n^{-3} )=$\vspace{1cm}\\ 
9)$(+9x^{2})(-7l^{3}++9z^{-4} )=$\vspace{1cm}\\ 
Realiza las siguientes multiplicaciones: \vspace{1cm}\\ 
10)$(+7b^{-4}-9e^{-4} )(-3f^{5}-3h^{2} )=$\vspace{1cm}\\ 
11)$(+9p^{4}-3u^{5} )(+7x^{-5}+6d^{-3} )=$\vspace{1cm}\\ 
12)$(+5b^{3}+7h^{3} )(+7v^{-2}+7w^{-3} )=$\vspace{1cm}\\ 

 \pagebreak 
Realiza las siguientes multiplicaciones: \vspace{1cm}\\ 
1)$(-2t)(-9k)=$\vspace{1cm}\\ 
2)$(+2a)(+8c)=$\vspace{1cm}\\ 
3)$(-7g)(+3z)=$\vspace{1cm}\\ 
Realiza las siguientes multiplicaciones: \vspace{1cm}\\ 
4)$(+9g^{4})(-5g^{2} )=$\vspace{1cm}\\ 
5)$(-8j^{2})(-3j^{-2} )=$\vspace{1cm}\\ 
6)$(-3a^{3})(+8a^{2} )=$\vspace{1cm}\\ 
Realiza las siguientes multiplicaciones: \vspace{1cm}\\ 
7)$(-3a^{-2})(+8i^{-2}+-3t^{5} )=$\vspace{1cm}\\ 
8)$(-6a^{3})(-3p^{-5}++2l^{-3} )=$\vspace{1cm}\\ 
9)$(-4k^{4})(+3q^{4}+-6p^{3} )=$\vspace{1cm}\\ 
Realiza las siguientes multiplicaciones: \vspace{1cm}\\ 
10)$(-3c^{5}-7i^{4} )(-2k^{-2}-6l^{-4} )=$\vspace{1cm}\\ 
11)$(+8e^{3}+9g^{-2} )(+5m^{5}+7b^{5} )=$\vspace{1cm}\\ 
12)$(+8z^{4}+3s^{4} )(-6i^{-2}+2k^{3} )=$\vspace{1cm}\\ 

 \pagebreak 
Realiza las siguientes multiplicaciones: \vspace{1cm}\\ 
1)$(-9x)(+9u)=$\vspace{1cm}\\ 
2)$(+5b)(+8r)=$\vspace{1cm}\\ 
3)$(-5r)(+3x)=$\vspace{1cm}\\ 
Realiza las siguientes multiplicaciones: \vspace{1cm}\\ 
4)$(-4u^{5})(-9u^{-2} )=$\vspace{1cm}\\ 
5)$(-7z^{3})(-3z^{4} )=$\vspace{1cm}\\ 
6)$(+2y^{4})(+6y^{-3} )=$\vspace{1cm}\\ 
Realiza las siguientes multiplicaciones: \vspace{1cm}\\ 
7)$(+6h^{3})(+7k^{3}+-2d^{-3} )=$\vspace{1cm}\\ 
8)$(+8p^{-5})(+2t^{4}++7s^{4} )=$\vspace{1cm}\\ 
9)$(-3a^{2})(-6q^{-2}+-3l^{5} )=$\vspace{1cm}\\ 
Realiza las siguientes multiplicaciones: \vspace{1cm}\\ 
10)$(+6c^{4}+8j^{4} )(+7y^{-2}+9o^{3} )=$\vspace{1cm}\\ 
11)$(-9x^{3}+6o^{-2} )(+2v^{-5}+8d^{2} )=$\vspace{1cm}\\ 
12)$(+8q^{2}-5g^{-5} )(+9r^{-4}+5h^{3} )=$\vspace{1cm}\\ 

 \pagebreak 
Realiza las siguientes multiplicaciones: \vspace{1cm}\\ 
1)$(-6b)(+9a)=$\vspace{1cm}\\ 
2)$(+9c)(-7l)=$\vspace{1cm}\\ 
3)$(-8i)(+8g)=$\vspace{1cm}\\ 
Realiza las siguientes multiplicaciones: \vspace{1cm}\\ 
4)$(+7e^{2})(+9e^{3} )=$\vspace{1cm}\\ 
5)$(+3e^{-5})(-4e^{3} )=$\vspace{1cm}\\ 
6)$(+5q^{-2})(+5q^{-4} )=$\vspace{1cm}\\ 
Realiza las siguientes multiplicaciones: \vspace{1cm}\\ 
7)$(+8j^{-5})(+5g^{-2}+-7a^{-2} )=$\vspace{1cm}\\ 
8)$(-5l^{-5})(+2z^{-4}+-6f^{5} )=$\vspace{1cm}\\ 
9)$(-8b^{-4})(+3z^{-2}+-8q^{5} )=$\vspace{1cm}\\ 
Realiza las siguientes multiplicaciones: \vspace{1cm}\\ 
10)$(+5v^{2}+7l^{2} )(-4h^{-2}+8y^{-5} )=$\vspace{1cm}\\ 
11)$(-6d^{5}+4j^{5} )(-4w^{3}+2o^{5} )=$\vspace{1cm}\\ 
12)$(-6j^{-5}-6c^{-3} )(-3i^{-3}-3h^{-2} )=$\vspace{1cm}\\ 

 \pagebreak 
Realiza las siguientes multiplicaciones: \vspace{1cm}\\ 
1)$(-7d)(-9v)=$\vspace{1cm}\\ 
2)$(+8s)(+7u)=$\vspace{1cm}\\ 
3)$(-8i)(+3o)=$\vspace{1cm}\\ 
Realiza las siguientes multiplicaciones: \vspace{1cm}\\ 
4)$(+2n^{5})(-5n^{2} )=$\vspace{1cm}\\ 
5)$(+5c^{-3})(-7c^{4} )=$\vspace{1cm}\\ 
6)$(-7a^{-5})(+9a^{2} )=$\vspace{1cm}\\ 
Realiza las siguientes multiplicaciones: \vspace{1cm}\\ 
7)$(-7w^{4})(-9y^{-2}+-2i^{-4} )=$\vspace{1cm}\\ 
8)$(+4c^{-5})(+8n^{2}++9q^{-5} )=$\vspace{1cm}\\ 
9)$(+8u^{2})(-2v^{-3}+-5m^{-3} )=$\vspace{1cm}\\ 
Realiza las siguientes multiplicaciones: \vspace{1cm}\\ 
10)$(+2r^{-4}-3j^{-5} )(-2n^{-3}+2c^{5} )=$\vspace{1cm}\\ 
11)$(-4n^{-2}-2b^{-4} )(+4v^{3}-9s^{-4} )=$\vspace{1cm}\\ 
12)$(+8x^{-2}+8f^{5} )(-9m^{4}-9z^{-5} )=$\vspace{1cm}\\ 

 \pagebreak 
\end{document}